Prove sub consistent using ordering

theories/syntactic_soundness.v
@@ -33,25 +33,52 @@ Definition tm_to_head (a : tm) :=
   | tJ _ _ _ _ => hBot
   end.
 
+Function hleq (a b : head) :=
+  match a, b with
+  | hBot , _ => true
+  | hPi, hPi => true
+  | hVoid, hVoid => true
+  | hNat, hNat => true
+  | hUniv, hUniv => true
+  | hEq, hEq => true
+  | _, _ => false
+  end.
+
+Notation "a \≤ b" := (hleq a b) (at level 60, no associativity).
+
+Lemma hleq_refl a : a \≤ a.
+Proof. elim : a=>//. Qed.
+
+Lemma hleq_trans a b c : a \≤ b -> b \≤ c -> a \≤ c.
+Proof. hauto q:on inv:head. Qed.
+
+Lemma hleq_antisym a b : a \≤ b -> b \≤ a -> a = b.
+Proof. hauto q:on inv:head. Qed.
+
 Lemma Par_head a b (h : a ⇒ b) :
-  forall hd, tm_to_head a = Some hd ->
-        tm_to_head b = Some hd.
+  tm_to_head a \≤ tm_to_head b.
 Proof. induction h => //. Qed.
 
 Lemma Par_head_star a b (h : a ⇒* b) :
-  forall hd, tm_to_head a = Some hd ->
-        tm_to_head b = Some hd.
-Proof. induction h; eauto using Par_head. Qed.
+  tm_to_head a \≤ tm_to_head b.
+Proof. induction h; eauto using Par_head, hleq_refl, hleq_trans.  Qed.
 
 Lemma Sub1_consistent A B (h : Sub1 A B) :
-  forall hd hd1, tm_to_head A = Some hd -> tm_to_head B = Some hd1 -> hd = hd1.
-Proof. elim : A B / h; scongruence. Qed.
+  tm_to_head A = tm_to_head B.
+Proof. elim : A B / h=>//. Qed.
+
+
+Lemma Sub_consistent' a b (h : a <: b) :
+  exists c, (tm_to_head a \≤ c) && (tm_to_head b \≤ c).
+Proof. hauto lq:on use:Par_head_star, Sub1_consistent b:on unfold:Sub. Qed.
+
+Lemma Sub_consistent_helper a b :
+  (exists c, (a \≤ c) && (b \≤ c)) -> (a \≤ b) || (b \≤ a).
+Proof. hauto qb:on inv:head. Qed.
 
 Lemma Sub_consistent a b (h : a <: b) :
-  forall hd hd1, tm_to_head a = Some hd ->
-            tm_to_head b = Some hd1 ->
-            hd = hd1.
-Proof. qblast use:Par_head_star, Sub1_consistent. Qed.
+  (tm_to_head a \≤ tm_to_head b) || (tm_to_head b \≤ tm_to_head a).
+Proof. auto using Sub_consistent', Sub_consistent_helper. Qed.
 
 (* -------------------------------------------------- *)
 
